@prefix rdf:     <http://www.w3.org/1999/02/22-rdf-syntax-ns#> .
@prefix rdfs:    <http://www.w3.org/2000/01/rdf-schema#> .
@prefix telepathy:     <http://nepomuk.kde.org/ontologies/2009/06/20/telepathy#> .
@prefix nao:     <http://www.semanticdesktop.org/ontologies/2007/08/15/nao#> .
@prefix nrl:     <http://www.semanticdesktop.org/ontologies/2007/08/15/nrl#> .
@prefix nco:     <http://www.semanticdesktop.org/ontologies/2007/03/22/nco#> .
@prefix xsd:     <http://www.w3.org/2001/XMLSchema#> .

telepathy: {telepathy:accountIdentifier
     a rdf:Property ;
          rdfs:subPropertyOf nao:identifier ;
          rdfs:comment "Identifier of a Local Telepathy Account (as given by the Telepathy Account Manaager).";
          rdfs:domain nco:IMAccount ;
          rdfs:label "accountIdentifier" ;
          rdfs:range xsd:string .

            telepathy:statusType
     a rdf:Property ;
          rdfs:comment "The current presence type as defined by the Telepathy Spec. Invalid values (by the Telepathy spec) should be considered as 0, Unset.";
          rdfs:domain nco:IMAccount ;
          rdfs:label "statusType" ;
          rdfs:range xsd:integer .

            telepathy:isBuddyOf
     a rdf:Property ;
          rdfs:comment "Indicates the local IM Account on whose buddy list this IM Account appears." ;
          rdfs:domain nco:IMAccount ;
          rdfs:label "isBuddyOf" ;
          rdfs:range nco:IMAccount .

          telepathy:avatarToken
     a rdf:Property ;
          rdfs:comment "The current avatar token for the nco:photo of this contact";
          rdfs:domain nco:Contact ;
          rdfs:label "avatarToken" ;
          rdfs:range xsd:string .

          telepathy:isBlocked
     a rdf:Property ;
          rdfs:comment "Indicates whether this account has been blocked by the user or not, if the protocol supports it." ;
          rdfs:domain nco:IMAccount ;
          rdfs:label "isBlocked" ;
          rdfs:range xsd:boolean .

          telepathy:publishesPresenceTo
     a rdf:Property ;
          rdfs:comment "Indicates to which local IM Accounts this IMAccount publishes presence to" ;
          rdfs:domain nco:IMAccount ;
          rdfs:label "publishesPresenceTo" ;
          rdfs:range nco:IMAccount .

          telepathy:requestedSubscriptionTo
     a rdf:Property ;
          rdfs:comment "Indicates to which local IM Accounts this IMAccount requested subscription to" ;
          rdfs:domain nco:IMAccount ;
          rdfs:label "requestedSubscriptionTo" ;
          rdfs:range nco:IMAccount .

          telepathy:IMCapability
    a rdfs:Class ;
          rdfs:label "IM Capabilities" ;
          rdfs:comment "Features of a certain IM connection (depends on the IMAccount implementation used by the Contact)" ;
          rdfs:subClassOf rdfs:Resource .

    telepathy:im-capability-text-chat a nco:IMCapability .
    telepathy:im-capability-media-calls a nco:IMCapability .
    telepathy:im-capability-audio-calls a nco:IMCapability .
    telepathy:im-capability-video-calls a nco:IMCapability .
    telepathy:im-capability-upgrading-calls a nco:IMCapability .
    telepathy:im-capability-file-transfers a nco:IMCapability .
    telepathy:im-capability-stream-tubes a nco:IMCapability .
    telepathy:im-capability-dbus-tubes a nco:IMCapability .

            telepathy:imCapability
    a rdf:Property ;
            rdfs:label "imContact Capability";
            rdfs:comment "Capabilities of an IM Contact, defining how can we interact with him";
            rdfs:domain nco:IMAccount ;
            rdfs:range nco:IMCapability .

}

<http://nepomuk.kde.org/ontologies/2009/06/20/telepathy/metadata>
{
    telepathy:
          a       nrl:DocumentGraph , nrl:Ontology ;
          nao:hasDefaultNamespace "http://nepomuk.kde.org/ontologies/2009/06/20/telepathy#" ;
          nao:hasDefaultNamespaceAbbreviation "telepathy" ;
          nao:lastModified "2009-06-20T20:46:32.866Z" ;
          nao:serializationLanguage "TriG" ;
          nao:status "Testing" ;
          nrl:updatable "0" ;
          nao:version "1" .

    <http://nepomuk.kde.org/ontologies/2009/06/20/telepathy/metadata>
          a       nrl:GraphMetadata , nrl:Ontology ;
          nao:serializationLanguage "TriG" ;
          nrl:coreGraphMetadataFor telepathy: .
}
